new/proof/github_com/goose_lang/goose/model/channel/logatom/chan_au_recv.v
@@ -4,7 +4,7 @@ From New.golang.theory Require Import lock.
 Require Export New.code.github_com.goose_lang.goose.model.channel.
 From New.generatedproof.github_com.goose_lang.goose Require Import model.channel.
 
-#[local] Transparent is_channel own_channel.
+#[local] Transparent IsChan OwnChan.
 
 Section atomic_specs.
 Context `{hG: heapGS Σ, !ffi_semantics _ _}.
@@ -15,8 +15,8 @@ Context `{!globalsGS Σ} {go_ctx : GoContext}.
 
 Local Lemma wp_TryReceive_blocking (ch: loc)  (γ: chan_names) :
   ∀ Φ ,
-  is_channel ch γ -∗
-  rcv_au_slow ch γ (λ v ok, Φ (#true, #v, #ok)%V) ∧ Φ (#false, #(default_val V), #true)%V -∗
+  IsChan ch γ -∗
+  RecvAU ch γ (λ v ok, Φ (#true, #v, #ok)%V) ∧ Φ (#false, #(default_val V), #true)%V -∗
   WP channel.Channel__TryReceiveⁱᵐᵖˡ #ch #t #true {{ Φ }}.
 Proof.
   iIntros (?) "Hch HΦ". iNamed "Hch".
@@ -31,7 +31,7 @@ Proof.
     iNamed "phys". iNamed "offer". wp_auto. unfold chan_cap_valid in Hcapvalid.
     wp_if_destruct.
     {
-      destruct buff as [|v rest].
+      destruct buffer as [|v rest].
       {
         iDestruct (own_slice_len with "slice") as "[%Hl %Hcap2]".
         rewrite length_nil in Hl.
@@ -39,18 +39,18 @@ Proof.
         word.
       }
       iLeft in "HΦ".
-      iAssert (own_channel ch (chan_rep.Buffered (v :: rest)) γ)%I
+      iAssert (OwnChan ch (chan_rep.Buffered (v :: rest)) γ)%I
         with "[Hchanrepfrag]" as "Hown".
       { iFrame. iPureIntro. unfold chan_cap_valid. done. }
       iMod (lc_fupd_elim_later with "[$] HΦ") as "HΦ".
-      unfold rcv_au_fast.
+      unfold NonBlockingRecvAU.
       iApply fupd_wp.
       iMod "HΦ".
       iMod (lc_fupd_elim_later with "[$] HΦ") as "HΦ".
       iNamed "HΦ".
-      iDestruct (own_channel_agree with "Hown Hoc") as %Heq.
+      iDestruct (OwnChan_agree with "Hown Hoc") as %Heq.
       subst s.
-      iMod (own_channel_halves_update (chan_rep.Buffered rest) with "Hown Hoc")
+      iMod (OwnChan_halves_update (chan_rep.Buffered rest) with "Hown Hoc")
         as "[Hown1 Hown2]".
       { simpl in *. lia. }
       iMod ("Hcont" with "Hown1") as "Hcont".
@@ -60,7 +60,7 @@ Proof.
       iDestruct (own_slice_elem_acc with "slice") as "[Hcell Hclose]".
       { exact Hpos. }
       { done. }
-      iSpecialize ("Hclose" $! v with "Hcell").  (* gives back [slice_val ↦* (v::draining)] *)
+      iSpecialize ("Hclose" $! v with "Hcell").  (* gives back [slice_val ↦* (v::buffer)] *)
       iDestruct (own_slice_len with "Hclose") as %(Hlen_eq & Hnonneg).
       assert (0 ≤ sint.Z (W64 0) < sint.Z slice_val.(slice.len_f)) as Hlt.
       { word. }
@@ -98,9 +98,9 @@ Proof.
       {
         word.
       }
-      assert (buff = []).
-      { destruct buff. { done. } { rewrite H in Hl. naive_solver. } }
-      subst buff.
+      assert (buffer = []).
+      { destruct buffer. { done. } { rewrite H in Hl. naive_solver. } }
+      subst buffer.
 
       wp_call.
       wp_apply (wp_lock_unlock
@@ -170,16 +170,16 @@ Proof.
       iNamed "phys". wp_auto_lc 5.
       iNamed "offer".
 
-      unfold rcv_au_inner.
+      unfold RecvNestedAU.
       iApply fupd_wp.
       iMod "Hau".
       iMod (lc_fupd_elim_later with "[$] Hau") as "HP".
       iNamed "HP".
-      iAssert (own_channel ch (chan_rep.SndCommit v0) γ)%I
+      iAssert (OwnChan ch (chan_rep.SndCommit v0) γ)%I
         with "[Hchanrepfrag]" as "Hown".
       { iFrame "∗#". iPureIntro. cbn [chan_cap_valid]. done. }
-      iDestruct (own_channel_agree with "[$Hocinner] [$Hown]") as "%Hseq". subst s.
-      iDestruct (own_channel_halves_update (chan_rep.Idle)
+      iDestruct (OwnChan_agree with "[$Hocinner] [$Hown]") as "%Hseq". subst s.
+      iDestruct (OwnChan_halves_update (chan_rep.Idle)
                   with "[$Hocinner] [$Hown]") as ">[Hgv1 Hgv2]".
       { done. }
       iMod ("Hcontinner" with "Hgv1") as "Hcont".
@@ -211,7 +211,7 @@ Proof.
     }
     {
       iNamed "phys". unfold chan_phys.
-      destruct draining.
+      destruct buffer.
       {
         iNamed "phys". wp_auto.
 
@@ -234,33 +234,33 @@ Proof.
     iNamed "phys". wp_auto.
     iNamed "offer".
     iApply "Hau" in "HP".
-    unfold send_au_slow.
+    unfold SendAU.
     iApply fupd_wp. iMod "HP".
     iMod (lc_fupd_elim_later with "[$] HP") as "HP". iNamed "HP".
     iDestruct "Hoc" as "(H1 & H2)".
     iDestruct (chan_rep_agree with "[$H1] [$Hchanrepfrag]") as "%Hseq". subst s.
-    iAssert (own_channel ch (chan_rep.Idle) γ)%I
+    iAssert (OwnChan ch (chan_rep.Idle) γ)%I
       with "[Hchanrepfrag]" as "Hown".
     { iFrame "∗#". iPureIntro. done. }
-    iAssert (own_channel ch (chan_rep.Idle) γ)%I
+    iAssert (OwnChan ch (chan_rep.Idle) γ)%I
       with "[H1]" as "Hown1".
     { iFrame. iPureIntro. done. }
-    iDestruct (own_channel_halves_update (chan_rep.SndPending v)
+    iDestruct (OwnChan_halves_update (chan_rep.SndPending v)
                 with "[$Hown] [$Hown1]") as ">[Hgv1 Hgv2]".
     { simpl in *. done. }
     iMod ("Hcont" with "Hgv2") as "Hcont1". iModIntro.
     iApply fupd_wp. iLeft in "HΦ". iMod "HΦ".
     iMod (lc_fupd_elim_later with "[$] HΦ") as "HP".
     iNamed "HP".
-    iDestruct (own_channel_agree with "[$Hgv1] [$Hoc]") as "%Hseq". subst s.
-    iDestruct (own_channel_halves_update (chan_rep.RcvCommit)
+    iDestruct (OwnChan_agree with "[$Hgv1] [$Hoc]") as "%Hseq". subst s.
+    iDestruct (OwnChan_halves_update (chan_rep.RcvCommit)
                 with "[$Hgv1] [$Hoc]") as ">[Hgv1 Hgv2]".
     { done. }
     iMod ("Hcont" with "Hgv2") as "Hcont". iModIntro.
     wp_call.
     wp_apply (wp_lock_unlock
                with "[$lock state v slice slice_cap buffer Hgv1 H2 Hpred Hoffer Hcont1 $Hlock]").
-    { unfold chan_inv_inner.  iExists (RcvDone v). iFrame "∗#".
+    { unfold chan_inv_inner.  iExists (RcvDone). iFrame "∗#".
       iNamed "Hgv1". iFrame.
     }
     done.
@@ -281,12 +281,13 @@ Proof.
   - iNamed "phys". wp_auto.
 
     wp_call.
+    iNamed "phys".
     wp_apply (wp_lock_unlock
                with "[$lock state v slice slice_cap buffer offer  $Hlock]").
-    { unfold chan_inv_inner. iExists (RcvDone v). iFrame. }
+    { unfold chan_inv_inner. iExists (RcvDone). iFrame. }
     iRight in "HΦ". iFrame.
   - iNamed "phys".
-    destruct draining.
+    destruct buffer.
     { iNamed "offer".
       unfold chan_logical.
       iNamed "phys".
@@ -294,7 +295,7 @@ Proof.
       iApply fupd_wp. iLeft in "HΦ". iMod "HΦ".
       iMod (lc_fupd_elim_later with "[$] HΦ") as "HΦ".
       iNamed "HΦ". unfold chan_logical. iDestruct "offer" as "[offer H]".
-      iDestruct (own_channel_agree with "[$offer] [$Hoc]") as "%Hseq". subst s.
+      iDestruct (OwnChan_agree with "[$offer] [$Hoc]") as "%Hseq". subst s.
 
       iMod ("Hcont" with "Hoc") as "Hcont". iModIntro.
       wp_if_destruct.
@@ -316,36 +317,36 @@ Proof.
       wp_if_destruct.
       {
         iLeft in "HΦ".
-        iAssert (own_channel ch (chan_rep.Closed (v :: draining)) γ)%I
+        iAssert (OwnChan ch (chan_rep.Closed (v :: buffer)) γ)%I
           with "[Hchanrepfrag]" as "Hown".
         { iFrame. iPureIntro. done. }
         iApply fupd_wp.
         iMod "HΦ".
         iMod (lc_fupd_elim_later with "[$] HΦ") as "HΦ".
         iNamed "HΦ".
-        iDestruct (own_channel_agree with "Hown Hoc") as %Heq.
+        iDestruct (OwnChan_agree with "Hown Hoc") as %Heq.
         subst s.
-        iMod (own_channel_halves_update (chan_rep.Closed draining) with "Hown Hoc")
+        iMod (OwnChan_halves_update (chan_rep.Closed buffer) with "Hown Hoc")
           as "[Hown1 Hown2]".
-        { simpl. destruct draining; [ done | ].
+        { simpl. destruct buffer; [ done | ].
           move: Hcapvalid; len.
         }
         iMod ("Hcont" with "Hown1") as "Hcont".
         iModIntro.
         have Hpos : 0 ≤ sint.Z (W64 0) by word.
-        have Hlookup0 : (v :: draining) !! 0%nat = Some v by done.
+        have Hlookup0 : (v :: buffer) !! 0%nat = Some v by done.
         iDestruct (own_slice_elem_acc with "slice") as "[Hcell Hclose]".
         { exact Hpos. }
         { done. }
-        iSpecialize ("Hclose" $! v with "Hcell").  (* gives back [slice_val ↦* (v::draining)] *)
+        iSpecialize ("Hclose" $! v with "Hcell").  (* gives back [slice_val ↦* (v::buffer)] *)
         iDestruct (own_slice_len with "Hclose") as %(Hlen_eq & Hnonneg).
         have Hlt : 0 ≤ sint.Z (W64 0) < sint.Z slice_val.(slice.len_f).
-        { move: Hlen_eq; simpl.  (* length (v::draining) = S (length draining) *)
+        { move: Hlen_eq; simpl.  (* length (v::buffer) = S (length buffer) *)
           (* sint.nat len = S _  ⇒  sint.Z len > 0 *)
           word. }
         wp_auto.
         wp_apply ((wp_load_slice_elem slice_val 0
-                     ( <[sint.nat (W64 0):=v]> (v :: draining)))
+                     ( <[sint.nat (W64 0):=v]> (v :: buffer)))
                    with "[Hclose]"). all: try word.
         { iFrame. done. }
         iIntros "Hsl". wp_auto.
@@ -355,7 +356,7 @@ Proof.
         wp_call.
         wp_apply (wp_lock_unlock
                    with "[$lock state slice_cap Hsl buffer Hown2  $Hlock]").
-        { unfold chan_inv_inner. iExists (Closed draining). iFrame.
+        { unfold chan_inv_inner. iExists (Closed buffer). iFrame.
 
           have -> : sint.nat (W64 0) = 0%nat by word.
           (* <[0:=v]>(<[0:=v]> [v]) = [v] *)
@@ -368,7 +369,7 @@ Proof.
           iDestruct (own_slice_cap_slice_f (slice_val) (W64 1) (DfracOwn 1)) as "H".
           { word. }
           iApply "H" in "slice_cap". iFrame.
-          destruct draining.
+          destruct buffer.
           { iFrame "∗#". iIntros "%Hcap". lia. }
           { iFrame. }
         }
@@ -389,8 +390,8 @@ Qed.
 
 Local Lemma wp_TryReceive_nonblocking (ch : loc)  (γ : chan_names) :
   ∀ Φ ,
-  is_channel ch γ -∗
-  rcv_au_fast ch γ (λ v ok, Φ (#true, #v, #ok)%V) (Φ (#false, #(default_val V), #true)%V) -∗
+  IsChan ch γ -∗
+  NonBlockingRecvAU ch γ (λ v ok, Φ (#true, #v, #ok)%V) (Φ (#false, #(default_val V), #true)%V) -∗
   WP channel.Channel__TryReceiveⁱᵐᵖˡ #ch #t #false {{ Φ }}.
 Proof.
   iIntros (?) "#Hch HΦ". iNamed "Hch".
@@ -408,16 +409,16 @@ Proof.
     iDestruct (own_slice_cap_wf with "slice_cap_inv") as %Hwf.
     wp_if_destruct.
     {
-      destruct buff as [|v rest].
+      destruct buffer as [|v rest].
       { simpl in *. word. }
       iLeft in "HΦ".
-      unfold rcv_au_fast.
+      unfold NonBlockingRecvAU.
       iApply fupd_wp.
       iMod "HΦ".
       iMod (lc_fupd_elim_later with "[$] HΦ") as "HΦ".
       iNamed "HΦ". iNamed "Hoc".
       iCombine "Hchanrepfrag Hchanrepfrag_inv" gives %[_ Heq]. subst.
-      iMod (own_channel_halves_update (chan_rep.Buffered rest) with "[$Hchanrepfrag_inv] [$Hchanrepfrag]")
+      iMod (OwnChan_halves_update (chan_rep.Buffered rest) with "[$Hchanrepfrag_inv] [$Hchanrepfrag]")
         as "[Hchanrepfrag Hchanrepfrag_inv]";
         [ (simpl in *; word) .. | ].
       iMod ("Hcont" with "Hchanrepfrag") as "Hcont".
@@ -440,9 +441,9 @@ Proof.
       done.
     }
     {
-      assert (buff = []).
-      { destruct buff; [done | simpl in *; word]. }
-      subst buff.
+      assert (buffer = []).
+      { destruct buffer; [done | simpl in *; word]. }
+      subst buffer.
       wp_call. iCombineNamed "*_inv" as "Hi".
       wp_apply (wp_lock_unlock
                  with "[$lock $Hlock Hi]").
@@ -461,7 +462,7 @@ Proof.
     iMod (lc_fupd_elim_later with "[$] HP_inv") as "HP_inv". iNamed "HP_inv".
     iNamed "Hoc".
     iDestruct (chan_rep_agree with "[$] [$]") as "%Hseq". subst s.
-    iDestruct (own_channel_halves_update (chan_rep.SndPending v)
+    iDestruct (OwnChan_halves_update (chan_rep.SndPending v)
                 with "[$Hchanrepfrag] [$Hchanrepfrag_inv]") as ">[Hchanrepfrag Hchanrepfrag_inv]";
       [done.. |].
     iMod ("Hcont" with "Hchanrepfrag") as "Hcont1_inv". iModIntro.
@@ -470,8 +471,8 @@ Proof.
     iMod "HΦ".
     iMod (lc_fupd_elim_later with "[$] HΦ") as "HΦ".
     iNamed "HΦ".
-    iDestruct (own_channel_agree with "[$] [$]") as "%Hseq". subst s.
-    iDestruct (own_channel_halves_update (chan_rep.RcvCommit)
+    iDestruct (OwnChan_agree with "[$] [$]") as "%Hseq". subst s.
+    iDestruct (OwnChan_halves_update (chan_rep.RcvCommit)
                 with "[$] [$]") as ">[Hchanrepfrag Hchanrepfrag_inv]".
     { done. }
 
@@ -480,7 +481,7 @@ Proof.
     wp_call. iCombineNamed "*_inv" as "Hi".
     wp_apply (wp_lock_unlock
                with "[$lock $Hlock Hi]").
-    { iNamed "Hi". unfold chan_inv_inner. iExists (RcvDone v). iFrame "∗#". }
+    { iNamed "Hi". unfold chan_inv_inner. iExists (RcvDone). iFrame "∗#". }
     done.
   - wp_auto_lc 2.
     wp_call. iCombineNamed "*_inv" as "Hi".
@@ -495,9 +496,9 @@ Proof.
   - wp_auto_lc 2.
     wp_call. iCombineNamed "*_inv" as "Hi".
     wp_apply (wp_lock_unlock with "[$lock $Hlock Hi]").
-    { iNamed "Hi". unfold chan_inv_inner. iExists (RcvDone _). iFrame. }
+    { iNamed "Hi". unfold chan_inv_inner. iExists (RcvDone). iFrame. }
     iRight in "HΦ". iFrame.
-  - destruct draining; iNamedSuffix "phys_inv" "_inv".
+  - destruct buffer; iNamedSuffix "phys_inv" "_inv".
     + simpl in *. iDestruct "offer_inv" as "[Hoc_inv Hoffer_inv]".
       wp_auto_lc 2.
       iDestruct (own_slice_len with "slice_inv") as %Hlen.
@@ -507,7 +508,7 @@ Proof.
       iMod (lc_fupd_elim_later with "[$] HΦ") as "HΦ".
       iNamed "HΦ".
       unfold chan_logical.
-      iDestruct (own_channel_agree with "[$Hoc_inv] [$Hoc]") as "%Hseq". subst s.
+      iDestruct (OwnChan_agree with "[$Hoc_inv] [$Hoc]") as "%Hseq". subst s.
 
       iMod ("Hcont" with "Hoc") as "Hcont". iModIntro.
 
@@ -525,11 +526,11 @@ Proof.
       iMod "HΦ".
       iMod (lc_fupd_elim_later with "[$] HΦ") as "HΦ".
       iNamed "HΦ". simpl. iDestruct "offer_inv" as "Hoc_inv".
-      iDestruct (own_channel_agree with "Hoc_inv Hoc") as %Heq.
+      iDestruct (OwnChan_agree with "Hoc_inv Hoc") as %Heq.
       subst s. iNamed "Hoc".
-      iMod (own_channel_halves_update (chan_rep.Closed draining) with "Hoc_inv [$Hchanrepfrag]")
+      iMod (OwnChan_halves_update (chan_rep.Closed buffer) with "Hoc_inv [$Hchanrepfrag]")
         as "[Hoc_inv Hoc]".
-      { simpl. destruct draining; [done|].
+      { simpl. destruct buffer; [done|].
         simpl in *. len. }
       { done. }
       iMod ("Hcont" with "Hoc") as "Hcont".
@@ -543,8 +544,8 @@ Proof.
       { iPureIntro. simpl in *. word. }
       wp_call. iCombineNamed "*_inv" as "Hi".
       wp_apply (wp_lock_unlock with "[$lock $Hlock Hi]").
-      { iNamed "Hi". unfold chan_inv_inner. iExists (Closed draining). iFrame.
-        destruct draining; iFrame "buffer_inv"; iFrame.
+      { iNamed "Hi". unfold chan_inv_inner. iExists (Closed buffer). iFrame.
+        destruct buffer; iFrame "buffer_inv"; iFrame.
         - iDestruct (own_slice_split_all (W64 1) with "slice_inv") as "[_ slice_inv]".
           { word. }
           rewrite drop_ge; last by len.
@@ -563,8 +564,8 @@ Qed.
 
 Local Lemma wp_TryReceive_nonblocking_alt (ch : loc) (γ : chan_names) :
   ∀ Φ ,
-  is_channel ch γ -∗
-  rcv_au_fast_alt ch γ (λ v ok, Φ (#true, #v, #ok)%V) (Φ (#false, #(default_val V), #true)%V) -∗
+  IsChan ch γ -∗
+  NonBlockingRecvAU_alt ch γ (λ v ok, Φ (#true, #v, #ok)%V) (Φ (#false, #(default_val V), #true)%V) -∗
   WP channel.Channel__TryReceiveⁱᵐᵖˡ #ch #t #false {{ Φ }}.
 Proof.
   iIntros (?) "#Hch HΦ". iNamed "Hch".
@@ -581,14 +582,14 @@ Proof.
     iDestruct (own_slice_len with "slice_inv") as %Hlen.
     iDestruct (own_slice_cap_wf with "slice_cap_inv") as %Hwf.
     wp_if_destruct.
-    + destruct buff as [|v rest].
+    + destruct buffer as [|v rest].
       { simpl in *. word. }
-      unfold rcv_au_fast.
+      unfold NonBlockingRecvAU.
       iApply fupd_wp. iMod "HΦ".
       iMod (lc_fupd_elim_later with "[$] HΦ") as "HΦ".
       iNamed "HΦ". iNamed "Hoc".
       iCombine "Hchanrepfrag Hchanrepfrag_inv" gives %[_ Heq]. subst.
-      iMod (own_channel_halves_update (chan_rep.Buffered rest) with "[$Hchanrepfrag_inv] [$Hchanrepfrag]")
+      iMod (OwnChan_halves_update (chan_rep.Buffered rest) with "[$Hchanrepfrag_inv] [$Hchanrepfrag]")
         as "[Hchanrepfrag Hchanrepfrag_inv]";
         [ (simpl in *; word) .. | ].
       iMod ("Hcont" with "Hchanrepfrag") as "Hcont".
@@ -609,9 +610,9 @@ Proof.
         word.
       }
       done.
-    + assert (buff = []).
-      { destruct buff; [done | simpl in *; word]. }
-      subst buff.
+    + assert (buffer = []).
+      { destruct buffer; [done | simpl in *; word]. }
+      subst buffer.
 
       iApply fupd_wp. iMod "HΦ".
       iMod (lc_fupd_elim_later with "[$] HΦ") as "HΦ".
@@ -649,7 +650,7 @@ Proof.
     iMod (lc_fupd_elim_later with "[$] HP_inv") as "HP_inv". iNamed "HP_inv".
     iNamed "Hoc".
     iDestruct (chan_rep_agree with "[$] [$]") as "%Hseq". subst s.
-    iDestruct (own_channel_halves_update (chan_rep.SndPending v)
+    iDestruct (OwnChan_halves_update (chan_rep.SndPending v)
                 with "[$Hchanrepfrag] [$Hchanrepfrag_inv]") as ">[Hchanrepfrag Hchanrepfrag_inv]";
       [done.. |].
     iMod ("Hcont" with "Hchanrepfrag") as "Hcont1_inv". iModIntro.
@@ -657,8 +658,8 @@ Proof.
     iMod "HΦ".
     iMod (lc_fupd_elim_later with "[$] HΦ") as "HΦ".
     iNamed "HΦ".
-    iDestruct (own_channel_agree with "[$] [$]") as "%Hseq". subst s.
-    iDestruct (own_channel_halves_update (chan_rep.RcvCommit)
+    iDestruct (OwnChan_agree with "[$] [$]") as "%Hseq". subst s.
+    iDestruct (OwnChan_halves_update (chan_rep.RcvCommit)
                 with "[$] [$]") as ">[Hchanrepfrag Hchanrepfrag_inv]".
     { done. }
 
@@ -667,7 +668,7 @@ Proof.
     wp_call. iCombineNamed "*_inv" as "Hi".
     wp_apply (wp_lock_unlock
                with "[$lock $Hlock Hi]").
-    { iNamed "Hi". unfold chan_inv_inner. iExists (RcvDone v). iFrame "∗#". }
+    { iNamed "Hi". unfold chan_inv_inner. iExists (RcvDone). iFrame "∗#". }
     done.
   - wp_auto_lc 2.
     iNamedSuffix "offer_inv" "_inv".
@@ -711,10 +712,10 @@ Proof.
     wp_call. iCombineNamed "*_inv" as "Hi".
     wp_apply (wp_lock_unlock
                with "[$lock $Hlock Hi]").
-    { iNamed "Hi". iFrame. unfold chan_inv_inner. iFrame. iExists (RcvDone _).
+    { iNamed "Hi". iFrame. unfold chan_inv_inner. iFrame. iExists (RcvDone).
       iFrame. iPureIntro. done. }
     iFrame.
-  - destruct draining; iNamedSuffix "phys_inv" "_inv".
+  - destruct buffer; iNamedSuffix "phys_inv" "_inv".
     + simpl in *. iDestruct "offer_inv" as "[Hoc_inv Hoffer_inv]".
       wp_auto_lc 2.
       iDestruct (own_slice_len with "slice_inv") as %Hlen.
@@ -724,7 +725,7 @@ Proof.
       iMod (lc_fupd_elim_later with "[$] HΦ") as "HΦ".
       iNamed "HΦ".
       unfold chan_logical.
-      iDestruct (own_channel_agree with "[$Hoc_inv] [$Hoc]") as "%Hseq". subst s.
+      iDestruct (OwnChan_agree with "[$Hoc_inv] [$Hoc]") as "%Hseq". subst s.
 
       iMod ("Hcont" with "Hoc") as "Hcont". iModIntro.
 
@@ -741,11 +742,11 @@ Proof.
       iMod "HΦ".
       iMod (lc_fupd_elim_later with "[$] HΦ") as "HΦ".
       iNamed "HΦ". simpl. iDestruct "offer_inv" as "Hoc_inv".
-      iDestruct (own_channel_agree with "Hoc_inv Hoc") as %Heq.
+      iDestruct (OwnChan_agree with "Hoc_inv Hoc") as %Heq.
       subst s. iNamed "Hoc".
-      iMod (own_channel_halves_update (chan_rep.Closed draining) with "Hoc_inv [$Hchanrepfrag]")
+      iMod (OwnChan_halves_update (chan_rep.Closed buffer) with "Hoc_inv [$Hchanrepfrag]")
         as "[Hoc_inv Hoc]".
-      { simpl. destruct draining; [done|].
+      { simpl. destruct buffer; [done|].
         simpl in *. len. }
       { done. }
       iMod ("Hcont" with "Hoc") as "Hcont".
@@ -759,8 +760,8 @@ Proof.
       { iPureIntro. simpl in *. word. }
       wp_call. iCombineNamed "*_inv" as "Hi".
       wp_apply (wp_lock_unlock with "[$lock $Hlock Hi]").
-      { iNamed "Hi". unfold chan_inv_inner. iExists (Closed draining). iFrame.
-        destruct draining; iFrame "buffer_inv"; iFrame.
+      { iNamed "Hi". unfold chan_inv_inner. iExists (Closed buffer). iFrame.
+        destruct buffer; iFrame "buffer_inv"; iFrame.
         - iDestruct (own_slice_split_all (W64 1) with "slice_inv") as "[_ slice_inv]".
           { word. }
           rewrite drop_ge; last by len.
@@ -779,13 +780,13 @@ Qed.
 
 Lemma wp_TryReceive (ch : loc) (γ : chan_names) (blocking : bool) :
   ∀ (Φ : val → iProp Σ),
-  is_channel ch γ -∗
-  (if blocking then rcv_au_slow ch γ (λ v ok, Φ (#true, #v, #ok)%V) ∧
+  IsChan ch γ -∗
+  (if blocking then RecvAU ch γ (λ v ok, Φ (#true, #v, #ok)%V) ∧
                     Φ (#false, #(default_val V), #true)%V
-   else (rcv_au_fast ch γ
+   else (NonBlockingRecvAU ch γ
            (λ v ok, Φ (#true, #v, #ok)%V)
            (Φ (#false, #(default_val V), #true)%V)
-           ∨ rcv_au_fast_alt ch γ
+           ∨ NonBlockingRecvAU_alt ch γ
                (λ v ok, Φ (#true, #v, #ok)%V)
                (Φ (#false, #(default_val V), #true)%V)
   )) -∗
@@ -801,12 +802,12 @@ Qed.
 
 Lemma wp_Receive (ch: loc) (γ: chan_names) :
   ∀ Φ,
-  is_channel ch γ -∗
-  (£1 ∗ £1 ∗ £1 ∗ £1 -∗ rcv_au_slow ch γ (λ v ok, Φ (#v, #ok)%V)) -∗
+  IsChan ch γ -∗
+  (£1 ∗ £1 ∗ £1 ∗ £1 -∗ RecvAU ch γ (λ v ok, Φ (#v, #ok)%V)) -∗
   WP channel.Channel__Receiveⁱᵐᵖˡ #ch #t #() {{ Φ }}.
 Proof.
   intros. iIntros "#Hic". iIntros "Hau".
-  iDestruct (is_channel_not_null with "[$Hic]") as "%Hnn".
+  iDestruct (IsChan_not_null with "[$Hic]") as "%Hnn".
   wp_call_lc "?".
   wp_auto_lc 3.
   iSpecialize ("Hau" with "[$]").
@@ -816,7 +817,7 @@ Proof.
   wp_apply (wp_TryReceive ch γ with "[$]").
   iSplit.
   { iFrame.
-    unfold rcv_au_slow. iMod "Hau".
+    unfold RecvAU. iMod "Hau".
     iModIntro. iModIntro. iNamed "Hau". iFrame.
     destruct s; try done.
     - destruct buff;first done.
@@ -824,7 +825,7 @@ Proof.
       iModIntro. wp_auto. wp_for_post.
       iFrame.
     - iIntros "H". iMod ("Hcont" with "H") as "H".
-      iModIntro. unfold rcv_au_inner.  iMod "H". iModIntro. iModIntro.
+      iModIntro. unfold RecvNestedAU.  iMod "H". iModIntro. iModIntro.
       iNamed "H".
       iFrame.
       destruct s; try done.
@@ -834,7 +835,7 @@ Proof.
         wp_for_post. done.
       }
       {
-        destruct draining; try done.
+        destruct drain; try done.
         iIntros "Hcontineer".
         iMod ("Hcontinner" with "Hcontineer") as "H". iModIntro. wp_auto.
         wp_for_post. done.
@@ -843,7 +844,7 @@ Proof.
     - iIntros "Hcontineer".
       iMod ("Hcont" with "Hcontineer") as "H". iModIntro. wp_auto.
       wp_for_post. done.
-    - destruct draining; try done.
+    - destruct drain; try done.
       {
         iIntros "Hcontineer".
         iMod ("Hcont" with "Hcontineer") as "H". iModIntro. wp_auto.
